coq/CoqOfSolidity/contracts/scl/mulmuladdX_fullgen_b4/run.v
@@ -1,157 +1,9 @@
 Require Import CoqOfSolidity.CoqOfSolidity.
+Require Import CoqOfSolidity.proofs.CoqOfSolidity.
 Require Import CoqOfSolidity.simulations.CoqOfSolidity.
+Require Import CoqOfSolidity.contracts.scl.mulmuladdX_fullgen_b4.contract_shallow.
 Import Stdlib.
-
-Module Contract_91.
-  (*
-    code {
-        {
-            /// @src 0:2011:14164  "contract Contract {..."
-            let _1 := memoryguard(0x80)
-            mstore(64, _1)
-            if callvalue() { revert(0, 0) }
-            let _2 := datasize("Contract_91_deployed")
-            codecopy(_1, dataoffset("Contract_91_deployed"), _2)
-            return(_1, _2)
-        }
-    }
-  *)
-  Definition code : M.t unit :=
-    let~ _1 := [[ memoryguard ~(| 0x80 |) ]] in
-    do~ [[
-      M.if_unit (| callvalue ~(||),
-        do~ [[ revert ~(| 0, 0 |) ]] in
-        M.pure tt
-      |)
-    ]] in
-    let~ _2 := [[ datasize ~(| Literal.string 0x436f6e74726163745f39315f6465706c6f796564000000000000000000000000 |) ]] in
-    do~ [[
-      codecopy ~(| _1, dataoffset ~(| Literal.string 0x436f6e74726163745f39315f6465706c6f796564000000000000000000000000 |), _2 |)
-    ]] in
-    do~ [[ return_ ~(| _1, _2 |) ]] in
-    M.pure tt.
-
-  Module Contract_91_deployed.
-    (*
-      function fun_ecGenMulmuladdX_store(var_Q_mpos, var_scalar_u, var_scalar_v) -> var_X
-      /// @ast-id 90
-      {
-          mstore(0x0140, var_Q_mpos)
-          mstore(0x0120, var_scalar_u)
-          mstore(0x0160, var_scalar_v)
-          mstore(0xa0, 0)
-          /// @ast-id 90
-          /** @ast-id 90 */ /** @ast-id 90 */ fun_ecGenMulmuladdX_store_2814()
-          /// @ast-id 90
-          /** @ast-id 90 */ var_X := /** @ast-id 90 */ /** @ast-id 90 */ mload(/** @ast-id 90 */ 0xa0)
-      }
-    *)
-    Definition fun_ecGenMulmuladdX_store (var_Q_mpos var_scalar_u var_scalar_v : U256.t) :
-        M.t U256.t :=
-      do~ [[ mstore ~(| 0x0140, var_Q_mpos |) ]] in
-      do~ [[ mstore ~(| 0x0120, var_scalar_u |) ]] in
-      do~ [[ mstore ~(| 0x0160, var_scalar_v |) ]] in
-      do~ [[ mstore ~(| 0xa0, 0 |) ]] in
-      do~ [[ fun_ecGenMulmuladdX_store_2814 ~(||) ]] in
-      do~ [[ mload ~(| 0xa0 |) ]] in
-      M.pure tt.
-
-    (*
-      code {
-          {
-              /// @src 0:2011:14164  "contract Contract {..."
-              let _1 := memoryguard(0x0200)
-              if iszero(lt(calldatasize(), 4))
-              {
-                  if eq(0x81a379ec, shr(224, calldataload(0)))
-                  {
-                      if callvalue() { revert(0, 0) }
-                      if slt(add(calldatasize(), not(3)), 384) { revert(0, 0) }
-                      if iszero(slt(35, calldatasize())) { revert(0, 0) }
-                      let newFreePtr := add(_1, 320)
-                      if or(gt(newFreePtr, 0xffffffffffffffff), lt(newFreePtr, _1))
-                      {
-                          mstore(0, shl(224, 0x4e487b71))
-                          mstore(4, 0x41)
-                          revert(0, 0x24)
-                      }
-                      mstore(64, newFreePtr)
-                      let dst := _1
-                      if gt(324, calldatasize()) { revert(0, 0) }
-                      let src := 4
-                      for { } lt(src, 324) { src := add(src, 0x20) }
-                      {
-                          mstore(dst, calldataload(src))
-                          dst := add(dst, 0x20)
-                      }
-                      let ret := fun_ecGenMulmuladdX_store(_1, calldataload(324), calldataload(356))
-                      let memPos := mload(64)
-                      mstore(memPos, ret)
-                      return(memPos, 0x20)
-                  }
-              }
-              revert(0, 0)
-          }
-    *)
-    Definition code :=
-      do~ [[
-        let~ _1 := [[ memoryguard ~(| 0x0200 |) ]] in
-        do~ [[
-          M.if_unit (| iszero ~(| lt ~(| calldatasize ~(||), 4 |) |),
-            [[
-              M.if_unit (| eq ~(| 0x81a379ec, shr ~(| 224, calldataload ~(| 0 |) |) |),
-                do~ [[
-                  M.if_unit (| callvalue ~(||),
-                    do~ [[ revert ~(| 0, 0 |) ]] in
-                    M.pure tt
-                  |)
-                ]] in
-                do~ [[
-                  M.if_unit (| slt ~(| add ~(| calldatasize ~(||), not ~(| 3 |) |), 384 |),
-                    do~ [[ revert ~(| 0, 0 |) ]] in
-                    M.pure tt
-                  |)
-                ]] in
-                do~ [[
-                  M.if_unit (| iszero ~(| slt ~(| 35, calldatasize ~(||) |) |),
-                    do~ [[ revert ~(| 0, 0 |) ]] in
-                    M.pure tt
-                  |)
-                ]] in
-                let~ newFreePtr := [[ add ~(| _1, 320 |) ]] in
-                do~ [[
-                  M.if_unit (| or ~(| gt ~(| newFreePtr, 0xffffffffffffffff |), lt ~(| newFreePtr, _1 |) |),
-                    do~ [[ mstore ~(| 0, shl ~(| 224, 0x4e487b71 |) |) ]] in
-                    do~ [[ mstore ~(| 4, 0x41 |) ]] in
-                    do~ [[ revert ~(| 0, 0x24 |) ]] in
-                    M.pure tt
-                  |)
-                ]] in
-                do~ [[ mstore ~(| 64, newFreePtr |) ]] in
-                let~ dst := [[ _1 ]] in
-                do~ [[
-                  M.if_unit (| gt ~(| 324, calldatasize ~(||) |),
-                    do~ [[ revert ~(| 0, 0 |) ]] in
-                    M.pure tt
-                  |)
-                ]] in
-                let~ src := [[ 4 ]] in
-                (* for loop: TODO *)
-                let~ ret := [[ fun_ecGenMulmuladdX_store ~(| _1, calldataload ~(| 324 |), calldataload ~(| 356 |) |) ]] in
-                let~ memPos := [[ mload ~(| 64 |) ]] in
-                do~ [[ mstore ~(| memPos, ret |) ]] in
-                do~ [[ return_ ~(| memPos, 0x20 |) ]] in
-                M.pure tt
-              |)
-            ]]
-          |)
-      ]] in
-      do~ [[ revert ~(| 0, 0 |) ]] in
-      M.pure tt
-    ]] in
-    M.pure tt.
-
-Ltac Zify.zify_post_hook ::= Z.to_euclidean_division_equations.
+Import RunO.
 
 Module Q.
   (* store Qx, Qy, Q'x, Q'y p, a, gx, gy, gx2pow128, gy2pow128  *)
@@ -169,253 +21,111 @@ Module Q.
   }.
 End Q.
 
-Module Curve.
-  Record t : Set := {
-    a : Z;
-    b : Z;
-  }.
-End Curve.
-
-Module Zp.
-  Module Valid.
-    Definition t (p n : Z) : Prop :=
-      0 <= n < p.
-  End Valid.
-End Zp.
-
-(** Affine points, excluding zero *)
-Module PA.
-  Record t : Set := {
-    X : U256.t;
-    Y : U256.t;
-  }.
-
-  Module Valid.
-    Record t (p : U256.t) (P : PA.t) : Prop := {
-      X : Zp.Valid.t p P.(PA.X);
-      Y : Zp.Valid.t p P.(PA.Y);
-    }.
-  End Valid.
-
-  Definition add (a p : Z) (P1 P2 : t) : option t :=
-    (* opposite *)
-    if (P1.(X) =? P2.(X)) && (P1.(Y) =? - P2.(Y)) then
-      None
-    (* double *)
-    else if (P1.(X) =? P2.(X)) && (P1.(Y) =? P2.(Y)) then
-      let lambda := (3 * P1.(X) ^ 2 + a) / (2 * P1.(Y)) in
-      let x := (lambda ^ 2 - 2 * P1.(X)) mod p in
-      Some {|
-        X := x;
-        Y := (lambda * (P1.(X) - x) - P1.(Y)) mod p;
-      |}
-    (* add *)
-    else
-      let lambda := (P2.(Y) - P1.(Y)) / (P2.(X) - P1.(X)) in
-      let x := (lambda ^ 2 - P1.(X) - P2.(X)) mod p in
-      Some {|
-        X := x;
-        Y := (lambda * (P1.(X) - x) - P1.(Y)) mod p;
-      |}.
-End PA.
-
-(** Points, with a dummy value for the zero *)
-Module P.
-  Definition t : Set :=
-    option PA.t.
-
-  Module Valid.
-    Definition t (p : U256.t) (P : P.t) : Prop :=
-      match P with
-      | None => True
-      | Some P => PA.Valid.t p P
-      end.
-  End Valid.
-
-  Definition zero : P.t :=
-    None.
-
-  Definition add (a p : Z) (P1 P2 : t) : t :=
-    match P1, P2 with
-    | None, P | P, None => P
-    | Some P1, Some P2 => PA.add a p P1 P2
-    end.
-
-  Lemma add_zero_l (a p : U256.t) (P : t) :
-    add a p zero P = P.
-  Proof.
-    reflexivity.
-  Qed.
-
-  Lemma add_zero_r (a p : U256.t) (P : t) :
-    add a p P zero = P.
-  Proof.
-    destruct P; reflexivity.
-  Qed.
-
-  Axiom add_commut :
-    forall (a p : U256.t) (P1 P2 : t),
-    add a p P1 P2 =
-    add a p P2 P1.
-
-  Axiom add_commut_nested :
-    forall (a p : U256.t) (P1 P2 P3 : t),
-    add a p (add a p P1 P2) P3 =
-    add a p (add a p P1 P3) P2.
-End P.
-
-(** Points in the ZZ, ZZZ representation *)
-Module PZZ.
-  Record t : Set := {
-    X : U256.t;
-    Y : U256.t;
-    ZZ : U256.t;
-    ZZZ : U256.t;
-  }.
-
-  Module Valid.
-    Record t (p : U256.t) (P : PZZ.t) : Prop := {
-      X : Zp.Valid.t p P.(PZZ.X);
-      Y : Zp.Valid.t p P.(PZZ.Y);
-      ZZ : Zp.Valid.t p P.(PZZ.ZZ);
-      ZZZ : Zp.Valid.t p P.(PZZ.ZZZ);
-      zero : P.(PZZ.ZZ) = 0 <-> P.(PZZ.ZZZ) = 0;
-    }.
-  End Valid.
-
-  Definition zero : PZZ.t := {|
-    PZZ.X := 0;
-    PZZ.Y := 0;
-    PZZ.ZZ := 0;
-    PZZ.ZZZ := 0;
-  |}.
-
-  Lemma zero_is_valid (p : U256.t)
-      (H_p : 2 <= p) :
-    Valid.t p zero.
-  Proof.
-    constructor; unfold Zp.Valid.t; simpl; lia.
-  Qed.
-
-  Definition of_PA (P : PA.t) : PZZ.t := {|
-    PZZ.X := P.(PA.X);
-    PZZ.Y := P.(PA.Y);
-    PZZ.ZZ := 1;
-    PZZ.ZZZ := 1;
-  |}.
-
-  Lemma of_PA_is_valid (p : U256.t) (P : PA.t)
-      (H_p : 2 <= p)
-      (H_P : PA.Valid.t p P) :
-    Valid.t p (of_PA P).
-  Proof.
-    destruct H_P; unfold Zp.Valid.t in *.
-    unfold of_PA.
-    constructor; unfold Zp.Valid.t; simpl; lia.
-  Qed.
-
-  Definition of_P (P : P.t) : PZZ.t :=
-    match P with
-    | None => zero
-    | Some P => of_PA P
-    end.
-
-  Lemma of_P_is_valid (p : U256.t) (P : P.t)
-      (H_p : 2 <= p < 2^256)
-      (H_P : P.Valid.t p P) :
-    Valid.t p (of_P P).
-  Proof.
-    destruct P as [P|].
-    { now apply of_PA_is_valid. }
-    { now apply zero_is_valid. }
-  Qed.
-
-  (** We do not need to check for [ZZZ] as both should be zero at the same time. *)
-  Definition is_zero (P : PZZ.t) : bool :=
-    P.(ZZ) =? 0.
-
-  Definition to_P (p : Z) (P : PZZ.t) : P.t :=
-    if is_zero P then
-      None
-    else
-      Some {|
-        PA.X := (P.(X) / P.(ZZ)) mod p;
-        PA.Y := (P.(Y) / P.(ZZZ)) mod p;
-      |}.
-
-  Lemma to_P_is_valid (p : U256.t) (P : PZZ.t)
-      (H_p : 2 <= p) :
-    P.Valid.t p (to_P p P).
-  Proof.
-    unfold P.Valid.t, to_P, is_zero; simpl.
-    destruct (ZZ P =? 0) eqn:H_ZZ_eq; simpl; [exact I|].
-    constructor; unfold Zp.Valid.t; simpl; lia.
-  Qed.
-
-  Lemma to_P_of_PA_eq (p : U256.t) (P : PA.t)
-      (H_P : PA.Valid.t p P) :
-    to_P p (of_PA P) = Some P.
-  Proof.
-    unfold to_P, of_PA; simpl.
-    destruct H_P; unfold Zp.Valid.t in *.
-    destruct P; simpl in *.
-    repeat f_equal.
-    all: rewrite Z.mod_small; lia.
-  Qed.
-
-  Lemma to_P_of_P_eq (p : U256.t) (P : P.t)
-      (H_P : P.Valid.t p P) :
-    to_P p (of_P P) = P.
-  Proof.
-    destruct P as [P|].
-    { apply to_P_of_PA_eq, H_P. }
-    { reflexivity. }
-  Qed.
-End PZZ.
-
-(*
-//normalized addition of two point, must not be neutral input
-function ecAddn2(x1, y1, zz1, zzz1, x2, y2, _p) -> _x, _y, _zz, _zzz {
-  y1 := sub(_p, y1)
-  y2 := addmod(mulmod(y2, zzz1, _p), y1, _p)
-  x2 := addmod(mulmod(x2, zz1, _p), sub(_p, x1), _p)
-  _x := mulmod(x2, x2, _p) //PP = P^2
-  _y := mulmod(_x, x2, _p) //PPP = P*PP
-  _zz := mulmod(zz1, _x, _p) ////ZZ3 = ZZ1*PP
-
-  _zzz := mulmod(zzz1, _y, _p) ////ZZZ3 = ZZZ1*PPP
-  zz1 := mulmod(x1, _x, _p) //Q = X1*PP
-  _x := addmod(addmod(mulmod(y2, y2, _p), sub(_p, _y), _p), mulmod(sub(_p,2), zz1, _p), _p) //R^2-PPP-2*Q
-
-  x1:=mulmod(addmod(zz1, sub(_p, _x), _p), y2, _p)//necessary split not to explose stack
-  _y := addmod(x1, mulmod(y1, _y, _p), _p) //R*(Q-X3)
-}
-*)
 Definition ecAddn2 (P1 : PZZ.t) (P2 : PA.t) (p : U256.t) : PZZ.t :=
-  let y1 := Pure.sub p P1.(PZZ.Y) in
-  let y2 := Pure.addmod (Pure.mulmod P2.(PA.Y) P1.(PZZ.ZZZ) p) y1 p in
-  let x2 := Pure.addmod (Pure.mulmod P2.(PA.X) P1.(PZZ.ZZ) p) (Pure.sub p P1.(PZZ.X)) p in
-  let _x := Pure.mulmod x2 x2 p in
-  let _y := Pure.mulmod _x x2 p in
-  let _zz := Pure.mulmod P1.(PZZ.ZZ) _x p in
+  let usr'dollar'x1 := P1.(PZZ.X) in
+  let usr'dollar'y1 := P1.(PZZ.Y) in
+  let usr'dollar'zz1 := P1.(PZZ.ZZ) in
+  let usr'dollar'zzz1 := P1.(PZZ.ZZZ) in
+  let usr'dollar'x2 := P2.(PA.X) in
+  let usr'dollar'y2 := P2.(PA.Y) in
+  let usr'dollar'_p := p in
 
-  let _zzz := Pure.mulmod P1.(PZZ.ZZZ) _y p in
-  let zz1 := Pure.mulmod P1.(PZZ.X) _x p in
-  let _x :=
+  let usr'dollar'y2_1 :=
     Pure.addmod
-      (Pure.addmod (Pure.mulmod y2 y2 p) (Pure.sub p _y) p)
-      (Pure.mulmod (Pure.sub p 2) zz1 p)
-      p in
-
-  let x1 := Pure.mulmod (Pure.addmod zz1 (Pure.sub p _x) p) y2 p in
-  let _y := Pure.addmod x1 (Pure.mulmod y1 _y p) p in
+      (Pure.mulmod usr'dollar'y2 usr'dollar'zzz1 usr'dollar'_p)
+      (Pure.sub usr'dollar'_p usr'dollar'y1)
+      usr'dollar'_p in
+  let usr'dollar'x2_1 :=
+    Pure.addmod
+      (Pure.mulmod usr'dollar'x2 usr'dollar'zz1 usr'dollar'_p)
+      (Pure.sub usr'dollar'_p usr'dollar'x1)
+      usr'dollar'_p in
+  let usr_x_1 :=
+    Pure.mulmod usr'dollar'x2_1 usr'dollar'x2_1 usr'dollar'_p in
+  let usr_y_1 :=
+    Pure.mulmod usr_x_1 usr'dollar'x2_1 usr'dollar'_p in
+  let usr_zz :=
+    Pure.mulmod usr'dollar'zz1 usr_x_1 usr'dollar'_p in
+  let usr_zzz :=
+    Pure.mulmod usr'dollar'zzz1 usr_y_1 usr'dollar'_p in
+  let usr'dollar'zz1_1 :=
+    Pure.mulmod usr'dollar'x1 usr_x_1 usr'dollar'_p in
+  let usr_x :=
+    Pure.addmod
+      (Pure.addmod
+        (Pure.mulmod usr'dollar'y2_1 usr'dollar'y2_1 usr'dollar'_p)
+        (Pure.sub usr'dollar'_p usr_y_1)
+        usr'dollar'_p)
+      (Pure.mulmod
+        (Pure.add usr'dollar'_p (Pure.not 1))
+        usr'dollar'zz1_1
+        usr'dollar'_p)
+      usr'dollar'_p in
+  let usr_y :=
+    Pure.addmod
+      (Pure.mulmod
+        (Pure.addmod
+          usr'dollar'zz1_1
+          (Pure.sub usr'dollar'_p usr_x)
+          usr'dollar'_p)
+        usr'dollar'y2_1
+        usr'dollar'_p)
+      (Pure.mulmod
+        (Pure.sub usr'dollar'_p usr'dollar'y1)
+        usr_y_1
+        usr'dollar'_p)
+      usr'dollar'_p in
 
   {|
-    PZZ.X := _x;
-    PZZ.Y := _y;
-    PZZ.ZZ := _zz;
-    PZZ.ZZZ := _zzz
+    PZZ.X := usr_x;
+    PZZ.Y := usr_y;
+    PZZ.ZZ := usr_zz;
+    PZZ.ZZZ := usr_zzz
   |}.
+
+Lemma run_usr'dollar'ecAddn2 codes environment state
+    (P1_X P1_Y P1_ZZ P1_ZZZ P2_X P2_Y : U256.t) (p : U256.t) :
+  let output :=
+    ecAddn2
+      {| PZZ.X := P1_X; PZZ.Y := P1_Y; PZZ.ZZ := P1_ZZ; PZZ.ZZZ := P1_ZZZ |}
+      {| PA.X := P2_X; PA.Y := P2_Y |}
+      p in
+  let output := Result.Ok (output.(PZZ.X), output.(PZZ.Y), output.(PZZ.ZZ), output.(PZZ.ZZZ)) in
+  {{? codes, environment, Some state |
+    Contract_91.Contract_91_deployed.usr'dollar'ecAddn2 P1_X P1_Y P1_ZZ P1_ZZZ P2_X P2_Y p ⇓
+    output
+  | Some state ?}}.
+Proof.
+  simpl.
+  unfold Contract_91.Contract_91_deployed.usr'dollar'ecAddn2.
+  l. {
+    repeat (l; [repeat cu; p|]).
+    p.
+  }
+  p.
+Qed.
+
+Lemma run_usr'dollar'ecAddn2_2189 codes environment state
+    (P1_X P1_Y P2_X P2_Y : U256.t) (p : U256.t) :
+  let output :=
+    ecAddn2
+      {| PZZ.X := P1_X; PZZ.Y := P1_Y; PZZ.ZZ := 1; PZZ.ZZZ := 1 |}
+      {| PA.X := P2_X; PA.Y := P2_Y |}
+      p in
+  let output := Result.Ok (output.(PZZ.X), output.(PZZ.Y), output.(PZZ.ZZ), output.(PZZ.ZZZ)) in
+  {{? codes, environment, Some state |
+    Contract_91.Contract_91_deployed.usr'dollar'ecAddn2_2189 P1_X P1_Y P2_X P2_Y p ⇓
+    output
+  | Some state ?}}.
+Proof.
+  simpl.
+  unfold Contract_91.Contract_91_deployed.usr'dollar'ecAddn2_2189.
+  l. {
+    repeat (l; [repeat cu; p|]).
+    p.
+  }
+  p.
+Qed.
 
 Module Ts.
   Definition t : Set := list PZZ.t.
@@ -587,6 +297,8 @@ Definition get_Ts (Q : Q.t) : list PZZ.t :=
   (* mstore4(mload(0x40), 1920, X,Y,ZZ,ZZZ) *)
   let Ts := Ts ++ [T] in
   Ts.
+
+
 
 (*
   {
@@ -817,6 +529,428 @@ Module MainLoop.
     |} in
     state.
 End MainLoop.
+
+Definition sim_fun_ecGenMulmuladdX_store_2814_beginning (Q : Q.t) (scalar_u scalar_v : U256.t) :
+    unit :=
+  (*
+    uint256 mask=1<<127;
+    /* I. precomputations phase */
+
+    if(scalar_u==0&&scalar_v==0){
+        return 0;
+    }
+  *)
+  let mask := 2 ^ 127 in
+  if (scalar_u =? 0) && (scalar_v =? 0) then
+    tt
+  else
+  let _modulusp := Q.(Q.p) in
+  let Ts := get_Ts Q in
+  tt.
+
+Ltac load_store_line :=
+  with_strategy opaque [ecAddn2] (
+    (* We do that to avoid an exponential increase of the output *)
+    try set (ecAddn2 _ _ _) in |- *;
+    l; [repeat (
+      c; [
+        p ||
+        apply_run_mload ||
+        apply_run_mstore ||
+        apply run_usr'dollar'ecAddn2 ||
+        apply run_usr'dollar'ecAddn2_2189
+      |];
+      CanonizeState.execute;
+      s
+    ); p|];
+    s;
+    try p
+  ).
+
+Lemma run_fun_ecGenMulmuladdX_store_2814_beginning codes environment state
+    (
+      mem0 mem1 mem3 mem4 mem5 mem6 mem7 mem8
+      mem12 mem13 mem14 :
+      U256.t
+    )
+    (Q : Q.t) (scalar_u scalar_v : U256.t) :
+  let memoryguard : U256.t := 0 in
+  let location_Q : U256.t := 32 * 15 in
+  let memory_start : list U256.t :=
+    [
+      mem0; mem1; memoryguard; mem3; mem4; mem5; mem6; mem7; mem8; scalar_u;
+      location_Q; scalar_v; mem12; mem13; mem14;
+      Q.(Q.Qx);
+      Q.(Q.Qy);
+      Q.(Q.Q'x);
+      Q.(Q.Q'y);
+      Q.(Q.p);
+      Q.(Q.a);
+      Q.(Q.gx);
+      Q.(Q.gy);
+      Q.(Q.gx2pow128);
+      Q.(Q.gy2pow128)
+    ] ++ List.repeat 0 200 in
+  let state_start :=
+      make_state environment state memory_start [] in
+  let memory_end : list U256.t :=
+    [1; 2; 3; 4; 5; 6] in
+  let state_end :=
+    make_state environment state memory_end [] in
+  (* let output := sim_fun_ecGenMulmuladdX_store_2814_beginning Q scalar_u scalar_v in *)
+  let output := Result.Ok tt in
+  {{? codes, environment, Some state_start |
+    Contract_91.Contract_91_deployed.fun_ecGenMulmuladdX_store_2814 ⇓
+    output
+  | Some state_end ?}}.
+Proof.
+  simpl.
+  unfold Contract_91.Contract_91_deployed.fun_ecGenMulmuladdX_store_2814.
+  l. {
+    repeat load_store_line.
+    l. {
+      unfold Shallow.if_, Pure.iszero.
+      instantiate (2 := Result.Ok (BlockUnit.Tt, if scalar_u =? 0 then _ else _)).
+      destruct (scalar_u =? 0); s; [|p].
+      load_store_line.
+    }
+    s.
+    lu.
+    match goal with
+    | |- context [Shallow.if_ ?condition] =>
+      replace condition with (Z.b2z ((scalar_u =? 0) && (scalar_v =? 0)))
+    end.
+    2: {
+      unfold Pure.iszero.
+      now repeat destruct (_ =? 0).
+    }
+    match goal with
+    | |- context [Shallow.if_ (Z.b2z ?condition)] =>
+      destruct condition eqn:H_u_v_eq; s
+    end.
+    { load_store_line. }
+    { repeat load_store_line.
+      l. {
+        change (Pure.shl 127 1) with (2 ^ Z.of_nat (128 - 1)).
+        set (index := 128%nat).
+        assert (H_index_le : (index <= 128)%nat) by lia.
+        assert (H_get_s :
+          forall i, Z.of_nat index <= i <= 127 -> get_s scalar_u scalar_v i = 0
+        ) by lia.
+        Ltac foo index word2 :=
+          let index := eval cbv in (Z.to_nat (index / 32)) in
+          eapply (Memory.update_at index word2);
+            try apply get_memory_make_state_eq;
+            [|reflexivity|];
+            unfold List.replace_nth;
+            CanonizeState.execute.
+        foo 0xe0 (
+          if (index =? 128)%nat then
+            0
+          else
+            get_s scalar_u scalar_v (Z.of_nat index)
+        ). {
+          reflexivity.
+        }
+        foo 0x01a0 (2 ^ (Z.of_nat index - 1)). {
+          reflexivity.
+        }
+        induction index.
+        { (* The base case, corresponding to a bit position of `-1`, is impossible to reach. *)
+          assert (H_u_v_zero :
+            (forall i, 0 <= i <= 127 -> get_s scalar_u scalar_v i = 0) ->
+            scalar_u = 0 /\ scalar_v = 0
+          ) by admit.
+          exfalso; lia.
+        }
+        { eapply LoopStep.
+          { (* for body *)
+            load_store_line.
+            destruct (index =? 127)%nat eqn:?; s.
+            { l. {
+                load_store_line.
+              }
+              load_store_line.
+            }
+            { 
+
+            }
+            l. {
+              load_store_line.
+            }
+            load_store_line.
+          }
+          {
+        }
+        eapply LoopStep.
+        { Compute (224 / 32). load_store_line.
+          l. {
+            load_store_line.
+          }
+          load_store_line.
+        }
+        { induction index.
+          { assert (H_u_v_zero :
+              (forall i, 0 <= i <= 127 -> get_s scalar_u scalar_v i = 0) ->
+              scalar_u = 0 /\ scalar_v = 0
+            ) by admit.
+            exfalso; lia.
+          }
+          { apply IHindex; clear IHindex.
+            { lia. }
+            { 
+
+            }
+          }
+        }
+          l. {
+            c. {
+              apply_run_mload.
+            }
+            cu; p.
+          }
+          s.
+          l. {
+            l. {
+              repeat (c; [
+                p ||
+                apply_run_mload
+              |]).
+              s.
+              c. {
+                match goal with
+                | |- context[mstore _ ?value] =>
+                  change value with (get_s scalar_u scalar_v (2 ^ 127))
+                end.
+                apply_run_mstore.
+              }
+              CanonizeState.execute.
+              p.
+            }
+            p.
+          }
+          s.
+          l. {
+              c. {
+                apply_run_mload.
+              }
+              s.
+              cu; s.
+              c. {
+                match goal with
+                | |- context[mstore _ ?value] =>
+                  change value with (2 ^ 126)
+                end.
+                apply_run_mstore.
+              }
+              CanonizeState.execute.
+              p.
+            }
+            s.
+            p.
+          }
+          { 
+
+          }
+
+        }
+        simpl in (Pure.shl _ _).
+        match goal with
+        | |- context[Pure.shl _ _] =>
+        end.
+        cbv in (Pure.shl _ _).
+        match goal with
+        end.
+        unfold Pure.shl.
+        generalize 127.
+        Compute 416 / 32.
+      }
+
+
+
+
+
+      Time with_strategy opaque [ecAddn2] do 10 load_store_line.
+      Time with_strategy opaque [ecAddn2] do 10 load_store_line.
+      Time with_strategy opaque [ecAddn2] do 10 load_store_line.
+      Time with_strategy opaque [ecAddn2] do 10 load_store_line.
+      Time with_strategy opaque [ecAddn2] do 10 load_store_line.
+      Time with_strategy opaque [ecAddn2] do 10 load_store_line.
+      Time with_strategy opaque [ecAddn2] repeat load_store_line.
+      repeat set (ecAddn2 _ _) in |- *.
+      set (ecAddn2 _ _) in |- *.
+      
+    repeat load_store_line.
+      l. {
+        c. {
+          apply_run_mload.
+        }
+        c. {
+          apply_run_mload.
+        }
+        c. {
+          apply run_usr'dollar'ecAddn2_2189.
+        }
+        p.
+      }
+      with_strategy opaque [ecAddn2] repeat load_store_line.
+      set (GA := {| PA.X := Q.(Q.gx); PA.Y := Q.(Q.gy) |}).
+      set (G'ZZ :=
+        {| PZZ.X := Q.(Q.gx2pow128); PZZ.Y := Q.(Q.gy2pow128); PZZ.ZZ := 1; PZZ.ZZZ := 1 |}).
+      l. {
+        c. {
+          apply_run_mload.
+        }
+        c. {
+          apply_run_mload.
+        }
+        c. {
+          apply_run_mload.
+        }
+        c. {
+          apply run_usr'dollar'ecAddn2_2189.
+        }
+        p.
+      }
+      with_strategy opaque [ecAddn2] repeat load_store_line.
+        }
+      }
+      Compute 
+      load_store_line.
+      load_store_line.
+      load_store_line.
+      load_store_line.
+      load_store_line.
+      load_store_line.
+      load_store_line.
+      load_store_line.
+      load_store_line.
+      load_store_line.
+      load_store_line.
+      load_store_line.
+      load_store_line.
+      load_store_line.
+      load_store_line.
+    
+    
+    
+      l. {
+        c. {
+          apply_run_mstore.
+        }
+        p.
+      }
+      CanonizeState.execute.
+      l. {
+        c. {
+          apply_run_mstore.
+        }
+        p.
+      }
+      CanonizeState.execute.
+      l. {
+        c. {
+          apply_run_mstore.
+        }
+        p.
+      }
+      CanonizeState.execute.
+      l. {
+        c. {
+          apply_run_mload.
+        }
+        p.
+      }
+      l. {
+        cu; s.
+        change (Pure.add 0 2048) with 2048.
+        c. {
+          apply_run_mstore.
+        }
+        CanonizeState.execute.
+        p.
+      }
+      l. {
+        cu; s.
+        c. {
+          apply_run_mload.
+        }
+        s.
+        cu; s.
+        c. {
+          apply_run_mload.
+        }
+        s.
+        c. {
+          apply_run_mstore.
+        }
+        CanonizeState.execute.
+        p.
+      }
+      l. {
+        c. {
+          apply_run_mload.
+        }
+        p.
+      }
+      (* let~ usr_modulusp := [[ mload ~(| add ~(| _2, 2080 |) |) ]] in *)
+      l. {
+        cu; s.
+        c. {
+          apply_run_mload.
+        }
+        p.
+      }
+      (* let~ _3 := [[ add ~(| mload ~(| 0x0140 |), 224 |) ]] in *)
+      l. {
+        c. {
+          apply_run_mload.
+        }
+        cu; p.
+      }
+      (* let~ _4 := [[ mload ~(| _3 |) ]] in *)
+      l. {
+        c. {
+          apply_run_mload.
+        }
+        p.
+      }
+      (* let~ _5 := [[ add ~(| mload ~(| 0x0140 |), 192 |) ]] in *)
+      l. {
+        c. {
+          apply_run_mload.
+        }
+        cu; p.
+      }
+      (* do~ [[ mstore ~(| add ~(| 128, _2 |), mload ~(| _5 |) |) ]] in *)
+        l; [repeat (
+          c; [
+            p ||
+            apply_run_mload ||
+            apply_run_mstore
+          |];
+          CanonizeState.execute;
+          s
+        )|].
+        match goal with
+        | |- context[]
+        end.
+        cu; s.
+        c. {
+          apply_run_mload.
+        }
+        c. {
+          apply_run_mstore.
+        }
+        CanonizeState.execute.
+        p.
+      }
+      (* let~ _6 := [[ add ~(| mload ~(| 0x0140 |), 160 |) ]] in *)
+    }
+    repeat (l; [repeat cu; p|]).
+    p.
+  }
+Qed.
 
 (*
 function ecGenMulmuladdX_store(
