coq/CoqOfSolidity/contracts/scl/mulmuladdX_fullgen_b4/curve.v
@@ -1,0 +1,205 @@
+Require Import CoqOfSolidity.CoqOfSolidity.
+
+Module Curve.
+  Record t : Set := {
+    a : Z;
+    b : Z;
+  }.
+End Curve.
+
+Module Zp.
+  Module Valid.
+    Definition t (p n : Z) : Prop :=
+      0 <= n < p.
+  End Valid.
+End Zp.
+
+(** Affine points, excluding zero *)
+Module PA.
+  Record t : Set := {
+    X : U256.t;
+    Y : U256.t;
+  }.
+
+  Module Valid.
+    Record t (p : U256.t) (P : PA.t) : Prop := {
+      X : Zp.Valid.t p P.(PA.X);
+      Y : Zp.Valid.t p P.(PA.Y);
+    }.
+  End Valid.
+
+  Definition add (a p : Z) (P1 P2 : t) : option t :=
+    (* opposite *)
+    if (P1.(X) =? P2.(X)) && (P1.(Y) =? - P2.(Y)) then
+      None
+    (* double *)
+    else if (P1.(X) =? P2.(X)) && (P1.(Y) =? P2.(Y)) then
+      let lambda := (3 * P1.(X) ^ 2 + a) / (2 * P1.(Y)) in
+      let x := (lambda ^ 2 - 2 * P1.(X)) mod p in
+      Some {|
+        X := x;
+        Y := (lambda * (P1.(X) - x) - P1.(Y)) mod p;
+      |}
+    (* add *)
+    else
+      let lambda := (P2.(Y) - P1.(Y)) / (P2.(X) - P1.(X)) in
+      let x := (lambda ^ 2 - P1.(X) - P2.(X)) mod p in
+      Some {|
+        X := x;
+        Y := (lambda * (P1.(X) - x) - P1.(Y)) mod p;
+      |}.
+End PA.
+
+(** Points, with a dummy value for the zero *)
+Module P.
+  Definition t : Set :=
+    option PA.t.
+
+  Module Valid.
+    Definition t (p : U256.t) (P : P.t) : Prop :=
+      match P with
+      | None => True
+      | Some P => PA.Valid.t p P
+      end.
+  End Valid.
+
+  Definition zero : P.t :=
+    None.
+
+  Definition add (a p : Z) (P1 P2 : t) : t :=
+    match P1, P2 with
+    | None, P | P, None => P
+    | Some P1, Some P2 => PA.add a p P1 P2
+    end.
+
+  Lemma add_zero_l (a p : U256.t) (P : t) :
+    add a p zero P = P.
+  Proof.
+    reflexivity.
+  Qed.
+
+  Lemma add_zero_r (a p : U256.t) (P : t) :
+    add a p P zero = P.
+  Proof.
+    destruct P; reflexivity.
+  Qed.
+
+  Axiom add_commut :
+    forall (a p : U256.t) (P1 P2 : t),
+    add a p P1 P2 =
+    add a p P2 P1.
+
+  Axiom add_commut_nested :
+    forall (a p : U256.t) (P1 P2 P3 : t),
+    add a p (add a p P1 P2) P3 =
+    add a p (add a p P1 P3) P2.
+End P.
+
+(** Points in the ZZ, ZZZ representation *)
+Module PZZ.
+  Record t : Set := {
+    X : U256.t;
+    Y : U256.t;
+    ZZ : U256.t;
+    ZZZ : U256.t;
+  }.
+
+  Module Valid.
+    Record t (p : U256.t) (P : PZZ.t) : Prop := {
+      X : Zp.Valid.t p P.(PZZ.X);
+      Y : Zp.Valid.t p P.(PZZ.Y);
+      ZZ : Zp.Valid.t p P.(PZZ.ZZ);
+      ZZZ : Zp.Valid.t p P.(PZZ.ZZZ);
+      zero : P.(PZZ.ZZ) = 0 <-> P.(PZZ.ZZZ) = 0;
+    }.
+  End Valid.
+
+  Definition zero : PZZ.t := {|
+    PZZ.X := 0;
+    PZZ.Y := 0;
+    PZZ.ZZ := 0;
+    PZZ.ZZZ := 0;
+  |}.
+
+  Lemma zero_is_valid (p : U256.t)
+      (H_p : 2 <= p) :
+    Valid.t p zero.
+  Proof.
+    constructor; unfold Zp.Valid.t; simpl; lia.
+  Qed.
+
+  Definition of_PA (P : PA.t) : PZZ.t := {|
+    PZZ.X := P.(PA.X);
+    PZZ.Y := P.(PA.Y);
+    PZZ.ZZ := 1;
+    PZZ.ZZZ := 1;
+  |}.
+
+  Lemma of_PA_is_valid (p : U256.t) (P : PA.t)
+      (H_p : 2 <= p)
+      (H_P : PA.Valid.t p P) :
+    Valid.t p (of_PA P).
+  Proof.
+    destruct H_P; unfold Zp.Valid.t in *.
+    unfold of_PA.
+    constructor; unfold Zp.Valid.t; simpl; lia.
+  Qed.
+
+  Definition of_P (P : P.t) : PZZ.t :=
+    match P with
+    | None => zero
+    | Some P => of_PA P
+    end.
+
+  Lemma of_P_is_valid (p : U256.t) (P : P.t)
+      (H_p : 2 <= p < 2^256)
+      (H_P : P.Valid.t p P) :
+    Valid.t p (of_P P).
+  Proof.
+    destruct P as [P|].
+    { now apply of_PA_is_valid. }
+    { now apply zero_is_valid. }
+  Qed.
+
+  (** We do not need to check for [ZZZ] as both should be zero at the same time. *)
+  Definition is_zero (P : PZZ.t) : bool :=
+    P.(ZZ) =? 0.
+
+  Definition to_P (p : Z) (P : PZZ.t) : P.t :=
+    if is_zero P then
+      None
+    else
+      Some {|
+        PA.X := (P.(X) / P.(ZZ)) mod p;
+        PA.Y := (P.(Y) / P.(ZZZ)) mod p;
+      |}.
+
+  Lemma to_P_is_valid (p : U256.t) (P : PZZ.t)
+      (H_p : 2 <= p) :
+    P.Valid.t p (to_P p P).
+  Proof.
+    unfold P.Valid.t, to_P, is_zero; simpl.
+    destruct (ZZ P =? 0) eqn:H_ZZ_eq; simpl; [exact I|].
+    constructor; unfold Zp.Valid.t; simpl; lia.
+  Qed.
+
+  Lemma to_P_of_PA_eq (p : U256.t) (P : PA.t)
+      (H_P : PA.Valid.t p P) :
+    to_P p (of_PA P) = Some P.
+  Proof.
+    unfold to_P, of_PA; simpl.
+    destruct H_P; unfold Zp.Valid.t in *.
+    destruct P; simpl in *.
+    repeat f_equal.
+    all: rewrite Z.mod_small; lia.
+  Qed.
+
+  Lemma to_P_of_P_eq (p : U256.t) (P : P.t)
+      (H_P : P.Valid.t p P) :
+    to_P p (of_P P) = P.
+  Proof.
+    destruct P as [P|].
+    { apply to_P_of_PA_eq, H_P. }
+    { reflexivity. }
+  Qed.
+End PZZ.
